Prefix: : <http://www.semanticweb.org/stappel/ontologies/2023/7/midlayer-energy-ontology/>
Prefix: dc: <http://purl.org/dc/elements/1.1/>
Prefix: owl: <http://www.w3.org/2002/07/owl#>
Prefix: rdf: <http://www.w3.org/1999/02/22-rdf-syntax-ns#>
Prefix: rdfs: <http://www.w3.org/2000/01/rdf-schema#>
Prefix: xml: <http://www.w3.org/XML/1998/namespace>
Prefix: xsd: <http://www.w3.org/2001/XMLSchema#>



Ontology: <http://www.semanticweb.org/stappel/ontologies/2023/7/midlayer-energy-ontology>

Import: <http://purl.obolibrary.org/obo/bfo/2.0/bfo.owl>
Import: <http://purl.obolibrary.org/obo/ro/releases/2023-02-22/ro.owl>

AnnotationProperty: <http://purl.obolibrary.org/obo/IAO_0000115>

    
AnnotationProperty: <http://purl.obolibrary.org/obo/IAO_0000118>

    
AnnotationProperty: <http://purl.obolibrary.org/obo/IAO_0000119>

    
AnnotationProperty: rdfs:label

    
Datatype: rdf:PlainLiteral

    
Datatype: xsd:string

    
ObjectProperty: <http://purl.obolibrary.org/obo/BFO_0000051>

    
ObjectProperty: <http://purl.obolibrary.org/obo/BFO_0000054>

    
ObjectProperty: <http://purl.obolibrary.org/obo/RO_0000052>

    
ObjectProperty: <http://purl.obolibrary.org/obo/RO_0002410>

    
ObjectProperty: <http://purl.obolibrary.org/obo/RO_0019001>

    
ObjectProperty: <http://purl.obolibrary.org/obo/RO_0019002>

    
ObjectProperty: MENO_01100

    Annotations: 
        <http://purl.obolibrary.org/obo/IAO_0000115> "",
        rdfs:label "base of"
    
    SubPropertyOf: 
        owl:topObjectProperty
    
    Domain: 
        <http://purl.obolibrary.org/obo/BFO_0000019>
    
    Range: 
        <http://purl.obolibrary.org/obo/BFO_0000016>
    
    
ObjectProperty: owl:topObjectProperty

   

Class: <http://purl.obolibrary.org/obo/BFO_0000015>

    
Class: <http://purl.obolibrary.org/obo/BFO_0000016>

    
Class: <http://purl.obolibrary.org/obo/BFO_0000017>

    
Class: <http://purl.obolibrary.org/obo/BFO_0000019>

    SubClassOf: 
        MENO_01100 some <http://purl.obolibrary.org/obo/BFO_0000016>
    
    
Class: <http://purl.obolibrary.org/obo/BFO_0000040>

    
Class: MENO_01001

    Annotations: 
        <http://purl.obolibrary.org/obo/IAO_0000115> "Energy is a generic term (superclass) for the various kinds of qualities that (a) enable the systematic description of processes that realize the dispositions of entities and (b) are (possibly indirectly) convertible into heat.",
        rdfs:label "energy"
    
    SubClassOf: 
        <http://purl.obolibrary.org/obo/BFO_0000019>,
        <http://purl.obolibrary.org/obo/RO_0000052> some <http://purl.obolibrary.org/obo/BFO_0000040>
    
    
Class: MENO_01002

    Annotations: 
        <http://purl.obolibrary.org/obo/IAO_0000115> "Energy transfer is a process in which a type of energy is decreased in one bearer and simultaneously either the same or some other type of energy is increased in another bearer.",
        rdfs:label "energy transfer"
    
    SubClassOf: 
        MENO_01004,
        <http://purl.obolibrary.org/obo/BFO_0000051> some MENO_01004
    
    
Class: MENO_01003

    Annotations: 
        <http://purl.obolibrary.org/obo/IAO_0000115> "Energy transformation is a process in which the amount of one type of energy is decreased, and simultaneously one or more other types of energy are increased.",
        rdfs:label "energy transformation"
    
    SubClassOf: 
        MENO_01004,
        <http://purl.obolibrary.org/obo/BFO_0000051> some MENO_01004
    
    
Class: MENO_01004

    Annotations: 
        <http://purl.obolibrary.org/obo/IAO_0000115> "Energy transfer or transformation process is a process that has energy transfer and/or energy transformation processes as part.",
        rdfs:label "energy transfer or transformation process"
    
    SubClassOf: 
        <http://purl.obolibrary.org/obo/BFO_0000015>,
        <http://purl.obolibrary.org/obo/RO_0002410> some MENO_01013,
        <http://purl.obolibrary.org/obo/RO_0019001> some MENO_01001
    
    DisjointWith: 
        MENO_01013
    
    
Class: MENO_01005

    Annotations: 
        <http://purl.obolibrary.org/obo/IAO_0000115> "Chemical energy is a form of energy that is stored in molecular bonds of a material entity.",
        rdfs:label "chemical energy"
    
    SubClassOf: 
        MENO_01001
    
    
Class: MENO_01006

    Annotations: 
        <http://purl.obolibrary.org/obo/IAO_0000115> "Electrical energy is a form of energy derived from the potential or kinetic energy of charged particles.",
        <http://purl.obolibrary.org/obo/IAO_0000119> "http://openenergy-platform.org/ontology/oeo/OEO_00000139",
        rdfs:label "electrical energy"
    
    SubClassOf: 
        MENO_01001
    
    
Class: MENO_01007

    Annotations: 
        <http://purl.obolibrary.org/obo/IAO_0000115> "Kinetic energy is a relational energy quality that stored in the movement of a
material entity relational/referring to a static frame of reference.",
        rdfs:label "kinetic energy"
    
    SubClassOf: 
        MENO_01001
    
    
Class: MENO_01008

    Annotations: 
        <http://purl.obolibrary.org/obo/IAO_0000115> "Rest energy is an energy quality that is stored matter without being usable, i.e. observable in processes. It resides simply in the mass of the ultimate particles and cannot be further explained.",
        rdfs:label "rest energy"
    
    SubClassOf: 
        MENO_01001
    
    
Class: MENO_01009

    Annotations: 
        <http://purl.obolibrary.org/obo/IAO_0000115> "Radiative energy is energy that photons possess and which is dependend on the frequency and wave length of the photon. Radiative energy is transferred as electromagnetic waves in radiation processes.",
        rdfs:label "readiative energy"
    
    SubClassOf: 
        MENO_01001
    
    
Class: MENO_01010

    Annotations: 
        <http://purl.obolibrary.org/obo/IAO_0000115> "Gravitational potential energy is a relational energy quality that is stored in the (elevated) position of a material entity relational/referring to the ground (e.g. the Earth's surface).",
        rdfs:label "gravitational potential energy"
    
    SubClassOf: 
        MENO_01001
    
    
Class: MENO_01011

    Annotations: 
        <http://purl.obolibrary.org/obo/IAO_0000115> "Heat is a form of energy that is transferred from a point of high temperature to a point of lower temperature, which occurs spontaneously via conduction, convection or radiation.",
        <http://purl.obolibrary.org/obo/IAO_0000118> "heat",
        rdfs:label "thermal energy"
    
    SubClassOf: 
        MENO_01001
    
    
Class: MENO_01013

    Annotations: 
        <http://purl.obolibrary.org/obo/IAO_0000115> "Energy decrease is a process which negatively regulates an energy quality which results in an decrease / reduction in the intensity or magnitude of that quality (characteristic).",
        rdfs:label "energy decrease"
    
    SubClassOf: 
        MENO_01021,
        <http://purl.obolibrary.org/obo/RO_0002410> some MENO_01004,
        <http://purl.obolibrary.org/obo/RO_0019002> some MENO_01001
    
    DisjointWith: 
        MENO_01004
    
    
Class: MENO_01014

    Annotations: 
        <http://purl.obolibrary.org/obo/IAO_0000115> "Energy increase is a process which positively regulates an energy quality which results in an increase \\/ rise in the intensity or magnitude of that quality (characteristic).",
        rdfs:label "energy increase"
    
    SubClassOf: 
        MENO_01021,
        <http://purl.obolibrary.org/obo/RO_0002410> some MENO_01013,
        <http://purl.obolibrary.org/obo/RO_0019001> some MENO_01001
    
    
Class: MENO_01020

    Annotations: 
        <http://purl.obolibrary.org/obo/IAO_0000115> "A field is a material entity without mass that is bearer of some type of energy.",
        rdfs:label "field"
    
    SubClassOf: 
        <http://purl.obolibrary.org/obo/BFO_0000040>
    
    
Class: MENO_01021

    Annotations: 
        rdfs:label "quality affecting process"
    
    SubClassOf: 
        <http://purl.obolibrary.org/obo/BFO_0000015>
    
    
Class: MENO_01030

    Annotations: 
        rdfs:label "disposition to perform work"
    
    SubClassOf: 
        <http://purl.obolibrary.org/obo/BFO_0000016>,
        <http://purl.obolibrary.org/obo/BFO_0000054> some MENO_01004
    
    
Class: MENO_01031

    Annotations: 
        rdfs:label "disposition to heat"
    
    SubClassOf: 
        <http://purl.obolibrary.org/obo/BFO_0000016>,
        <http://purl.obolibrary.org/obo/BFO_0000054> some MENO_01004
    
    
Class: MENO_01040

    Annotations: 
        rdfs:label "radiation"
    
    SubClassOf: 
        MENO_01002
    
    
Class: MENO_01041

    Annotations: 
        rdfs:label "conduction"
    
    SubClassOf: 
        MENO_01002
    
    
Class: MENO_01042

    Annotations: 
        rdfs:label "convection"
    
    SubClassOf: 
        MENO_01002
    
    
Class: MENO_01043

    Annotations: 
        rdfs:label "combustion"
    
    SubClassOf: 
        MENO_01003
    
    
Class: MENO_01044

    Annotations: 
        rdfs:label "photosynthesis"
    
    SubClassOf: 
        MENO_01003
    
    
Class: MENO_01045

    Annotations: 
        rdfs:label "falling"
    
    SubClassOf: 
        MENO_01003
    
    
